Tealeaves/Examples/JAR/TranslateDemo.v
@@ -2,6 +2,9 @@ From Tealeaves.Examples Require Import Lambda.Confluence.
 From Tealeaves.Backends Require Import LN DB.
 From Tealeaves.Backends.Adapters Require Import LNtoDB DBtoLN Roundtrips.LNDB.
 
+Import List.ListNotations.
+
+Check LNtokey: lam LN -> key.
 Check toLN: key -> lam nat -> option (lam LN).
 Check toDB: key -> lam LN  -> option (lam nat).
 
@@ -11,27 +14,58 @@ Definition z: atom := 2.
 Definition a: atom := 3.
 Definition b: atom := 4.
 
-Example term1: lam LN := app (tvar (Bd 0)) (tvar (Fr x)).
-Example term2: lam LN := abs (app (tvar (Bd 0)) (tvar (Fr x))).
-Example term3: lam LN := abs (app (tvar (Fr z)) (tvar (Fr x))).
-Example term4: lam LN := abs (app (abs (abs (app (tvar (Fr z)) (tvar (Fr x))))) (app (tvar (Fr y)) (tvar (Fr a)))).
+Module de_bruijn.
 
-Import List.ListNotations.
+  Example term1: lam nat := app (tvar 0) (tvar 1).
+  Example term2: lam nat := abs (app (tvar 0) (tvar 1)).
+  Example term3: lam nat := app (abs (app (tvar 1) (tvar 0))) (app (tvar 1) (tvar 0)).
+  (* ^ example from paper *)
 
-Example k: key := [b; z; a; y; x].
+  Example k: key := [x ; y].
 
-Compute toDB k term1.
-Compute map (toLN k) (toDB k term1).
+  Compute toLN k term1.
+  Compute map (toDB k) (toLN k term1).
 
-Compute toDB k term2.
-Compute map (toLN k) (toDB k term2).
+  Compute toLN k term2.
+  Compute map (toDB k) (toLN k term2).
 
-Compute toDB k term3.
-Compute map (toLN k) (toDB k term3).
+  Compute toLN k term3.
+  Compute map (toDB k) (toLN k term3).
 
-Compute toDB k term4.
-Compute map (toLN k) (toDB k term4).
+End de_bruijn.
 
-Goal map (toLN k) (toDB k term4) = Some (Some term4).
-  reflexivity.
-Qed.
+Module locally_nameless.
+
+  Example term1: lam LN := app (tvar (Bd 0)) (tvar (Fr x)).
+  Example term2: lam LN := abs (app (tvar (Bd 0)) (tvar (Fr x))).
+  Example term3: lam LN := abs (app (tvar (Fr z)) (tvar (Fr x))).
+  Example term4: lam LN :=
+    abs (app
+           (abs (abs (app
+                        (tvar (Fr z))
+                        (tvar (Fr x)))))
+           (app
+              (tvar (Fr y))
+              (tvar (Fr a)))).
+
+  Import List.ListNotations.
+
+  Example k: key := [b; z; a; y; x].
+
+  Compute toDB k term1.
+  Compute map (toLN k) (toDB k term1).
+
+  Compute toDB k term2.
+  Compute map (toLN k) (toDB k term2).
+
+  Compute toDB k term3.
+  Compute map (toLN k) (toDB k term3).
+
+  Compute toDB k term4.
+  Compute map (toLN k) (toDB k term4).
+
+  Goal map (toLN k) (toDB k term4) = Some (Some term4).
+    reflexivity.
+  Qed.
+
+End locally_nameless.
